Simplified rules...

Gt3/JEq/Basic.lean
@@ -107,16 +107,12 @@ inductive Ctx.JEq : Ctx → Tm 0 → Tm 0 → Tm 0 → Prop
     (rhs_wf : JEq Γ Ba ba ba)
     (hba : JEq Γ Ba (b.lst a) ba)
     : JEq Γ Ba (.app (A.abs b) a) ba
-  | beta_fst' {Γ}  {A : Tm 0} {B : Tm 1} {a b : Tm 0} {m n} {L : Finset String}
-    (hA : JEq Γ (.univ m) A A)
-    (hB : ∀ x ∉ L, JEq (Γ.cons x A) (.univ n) (B.open x) (B.open x))
+  | beta_fst' {Γ}  {A : Tm 0} {B : Tm 1} {a b : Tm 0}
     (hp : JEq Γ (.sigma A B) (.pair a b) (.pair a b))
     (lhs_wf : JEq Γ A (.fst (.pair a b)) (.fst (.pair a b)))
     (rhs_wf : JEq Γ A a a)
     : JEq Γ A (.fst (.pair a b)) a
-  | beta_snd' {Γ}  {A : Tm 0} {B : Tm 1} {a b Ba : Tm 0} {m n} {L : Finset String}
-    (hA : JEq Γ (.univ m) A A)
-    (hB : ∀ x ∉ L, JEq (Γ.cons x A) (.univ n) (B.open x) (B.open x))
+  | beta_snd' {Γ}  {A : Tm 0} {B : Tm 1} {a b Ba : Tm 0}
     (hp : JEq Γ (.sigma A B) (.pair a b) (.pair a b))
     (lhs_wf : JEq Γ Ba (.snd (.pair a b)) (.snd (.pair a b)))
     (rhs_wf : JEq Γ Ba b b)
